src/array/FArray.v
@@ -1,34 +1,62 @@
-Require Import SetoidList Bool.
+Require Import SetoidList Bool OrderedType OrdersLists RelationPairs Orders.
 (* Require Import List Bool NArith Psatz Int63. *)
+Require Import RelationClasses.
 
-Section Array.
 
-  Class DecType T := {
-    eq_refl : forall x : T, x = x;
-    eq_sym : forall x y : T, x = y -> y = x;
-    eq_trans : forall x y z : T, x = y -> y = z -> x = z;
-    eq_dec : forall x y : T, { x = y } + { x <> y }
-  }.
+Class DecType T := {
+ eq_refl : forall x : T, x = x;
+ eq_sym : forall x y : T, x = y -> y = x;
+ eq_trans : forall x y z : T, x = y -> y = z -> x = z;
+ eq_dec : forall x y : T, { x = y } + { x <> y }
+}.
+
+Hint Immediate eq_sym.
+Hint Resolve eq_refl eq_trans.
+
+Class OrdType T := {
+  lt: T -> T -> Prop;
+  lt_trans : forall x y z : T, lt x y -> lt y z -> lt x z;
+  lt_not_eq : forall x y : T, lt x y -> ~ eq x y
+  (* compare : forall x y : T, Compare lt eq x y *)
+}.
+
+
+Hint Resolve lt_not_eq lt_trans.
+
+(* Global Instance Comparable T `(OrdType T) : *)
+
+Class Comparable T {ot:OrdType T} := {
+  compare : forall x y : T, Compare lt eq x y
+}.
+
+
+Set Implicit Arguments.
+
+
+
+Module Raw.
   
-  Hint Immediate eq_sym.
-  Hint Resolve eq_refl eq_trans.
-    
+  Section Array.
+
+  
   Variable key : Type.
   Variable elt : Type.
   Variable key_dec : DecType key.
+  Variable key_ord : OrdType key.
+  Variable key_comp : Comparable key.
   Variable elt_dec : DecType elt.
+  Variable elt_ord : OrdType elt.
 
-  Set Implicit Arguments.
 
-
+  
   Definition eqb_key (x y : key) : bool := if eq_dec x y then true else false.
   Definition eqb_elt (x y : elt) : bool := if eq_dec x y then true else false.
 
   Lemma eqb_key_eq x y : eqb_key x y = true <-> x = y.
-  Proof. unfold eqb_key. case (eq_dec x y); easy. Qed.
+  Proof. unfold eqb_key. case (eq_dec x y); split; easy. Qed.
 
   Lemma eqb_elt_eq x y : eqb_elt x y = true <-> x = y.
-  Proof. unfold eqb_elt. case (eq_dec x y); easy. Qed.
+  Proof. unfold eqb_elt. case (eq_dec x y); split; easy. Qed.
 
   Hint Immediate eqb_key_eq eqb_elt_eq.
   
@@ -38,10 +66,115 @@ Section Array.
   Definition eqe (a b : (key * elt)) := snd a = snd b.
   Definition eqke (a b : (key * elt)) := fst a = fst b /\ snd a = snd b.
 
-  Hint Unfold eqk eqke.
+  Definition ltk (a b : (key * elt)) := lt (fst a) (fst b).
+
+  (* Definition ltke (a b : (key * elt)) := *)
+  (*   lt (fst a) (fst b) \/ ( (fst a) = (fst b) /\ lt (snd a) (snd b)). *)
+  
+  Hint Unfold ltk (* ltke *) eqk eqke.
   Hint Extern 2 (eqke ?a ?b) => split.
 
+
+  Global Instance StrictOrder_OrdType T `(OrdType T) :
+    StrictOrder (lt : T -> T -> Prop).
+  Proof.
+    split.
+    unfold Irreflexive, Reflexive, complement.
+    intros. apply lt_not_eq in H0; auto.
+    unfold Transitive. intros x y z. apply lt_trans.
+  Qed.
   
+  Global Instance lt_key_strorder : StrictOrder (lt : key -> key -> Prop).
+  Proof. apply StrictOrder_OrdType. Qed.
+
+  Global Instance lt_elt_strorder : StrictOrder (lt : elt -> elt -> Prop).
+  Proof. apply StrictOrder_OrdType. Qed.
+
+  
+  Global Instance ke_dec : DecType (key * elt).
+  Proof.
+    split; auto.
+    intros; destruct x, y, z.
+    inversion H. inversion H0. trivial.
+    intros; destruct x, y.
+    destruct (eq_dec k k0).
+    destruct (eq_dec e e0).
+    left; rewrite e1, e2; auto.
+    right; unfold not in *. intro; inversion H. exact (n H2).
+    right; unfold not in *. intro; inversion H. exact (n H1).
+  Qed.
+
+  Global Instance ke_ord: OrdType (key * elt).
+  Proof.
+    exists ltk; unfold ltk; intros.
+    apply (lt_trans _ (fst y)); auto.
+    destruct x, y. simpl in H.
+    unfold not. intro. inversion H0.
+    apply (lt_not_eq k k0); auto.
+  Qed.
+
+
+  (* ltk ignore the second components *)
+
+   Lemma ltk_right_r : forall x k e e', ltk x (k,e) -> ltk x (k,e').
+   Proof. auto. Qed.
+
+   Lemma ltk_right_l : forall x k e e', ltk (k,e) x -> ltk (k,e') x.
+   Proof. auto. Qed.
+   Hint Immediate ltk_right_r ltk_right_l.
+
+
+  
+  
+  Notation Sort := (sort ltk).
+  Notation Inf := (lelistA (ltk)).
+  
+  Definition MapsTo (k:key)(e:elt):= InA eqke (k,e).
+  Definition In k m := exists e:elt, MapsTo k e m.
+
+  Notation NoDupA := (NoDupA eqk).
+
+  Hint Unfold MapsTo In.
+
+  
+  (* Instance ke_ord: OrdType (key * elt). *)
+  (* Proof. *)
+  (*   exists ltke. *)
+  (*   unfold ltke. intros. *)
+  (*   destruct H, H0. *)
+  (*   left; apply (lt_trans _ (fst y)); auto. *)
+  (*   destruct H0. left. rewrite <- H0. assumption. *)
+  (*   destruct H. left. rewrite H. assumption. *)
+  (*   destruct H, H0. *)
+  (*   right. split. *)
+  (*   apply (eq_trans _ (fst y)); trivial. *)
+  (*   apply (lt_trans _ (snd y)); trivial. *)
+  (*   unfold ltke. intros. *)
+  (*   destruct x, y. simpl in H. *)
+  (*   destruct H. *)
+  (*   apply lt_not_eq in H. *)
+  (*   unfold not in *. intro. inversion H0. apply H. trivial. *)
+  (*   destruct H. apply lt_not_eq in H0. unfold not in *. intro.  *)
+  (*   inversion H1. apply H0; trivial. *)
+  (*   intros. *)
+  (*   unfold ltke. *)
+  (*   destruct (compare (fst x) (fst y)). *)
+  (*   apply LT. left; assumption. *)
+  (*   destruct (compare (snd x) (snd y)). *)
+  (*   apply LT. right; split; assumption. *)
+  (*   apply EQ. destruct x, y. simpl in *. rewrite e, e0; trivial. *)
+  (*   apply GT. right; symmetry in e; split; assumption. *)
+  (*   apply GT. left; assumption. *)
+  (* Qed. *)
+
+  
+  (* Hint Immediate ke_ord. *)
+  (* Let ke_ord := ke_ord. *)
+
+  (* Instance keyelt_ord: OrdType (key * elt). *)
+
+
+  (* Variable keyelt_ord : OrdType (key * elt). *)
    (* eqke is stricter than eqk *)
 
    Lemma eqke_eqk : forall x x', eqke x x' -> eqk x x'.
@@ -70,16 +203,112 @@ Section Array.
   Proof.
     unfold eqke; intuition; [ eauto | congruence ].
   Qed.
+   
+  Lemma ltk_trans : forall e e' e'', ltk e e' -> ltk e' e'' -> ltk e e''.
+  Proof. eauto. Qed.
+
+  Lemma ltk_not_eqk : forall e e', ltk e e' -> ~ eqk e e'.
+  Proof. unfold ltk, eqk. intros. apply lt_not_eq; auto. Qed.
+
+  Lemma ltk_not_eqke : forall e e', ltk e e' -> ~eqke e e'.
+  Proof.
+    unfold eqke, ltk; intuition; simpl in *; subst.
+    apply lt_not_eq in H. auto.
+  Qed.
+  
 
   Hint Resolve eqk_trans eqke_trans eqk_refl eqke_refl.
+  Hint Resolve ltk_trans ltk_not_eqk ltk_not_eqke.
   Hint Immediate eqk_sym eqke_sym.
 
+
+  
   Global Instance eqk_equiv : Equivalence eqk.
   Proof. split; eauto. Qed.
 
   Global Instance eqke_equiv : Equivalence eqke.
   Proof. split; eauto. Qed.
 
+
+
+  Global Instance ltk_strorder : StrictOrder ltk.
+  Proof.
+    split.
+    unfold Irreflexive, Reflexive, complement.
+    intros. apply lt_not_eq in H; auto.
+    unfold Transitive. intros x y z. apply lt_trans.
+  Qed.
+
+
+  (* Instance ltke_strorder : StrictOrder ltke. *)
+  (* Proof. *)
+  (*   split. *)
+  (*   unfold Irreflexive, Reflexive, complement. *)
+  (*   intros. apply lt_not_eq in H; auto. *)
+  (*   unfold Transitive. apply lt_trans. *)
+  (* Qed. *)
+
+  Global Instance eq_equiv : @Equivalence (key * elt) eq.
+  Proof.
+    split; auto.
+    unfold Transitive. apply eq_trans.
+  Qed.
+    
+  (* Instance ltke_compat : Proper (eq ==> eq ==> iff) ltke. *)
+  (* Proof. *)
+  (*   split; rewrite H, H0; trivial. *)
+  (* Qed. *)
+    
+  Global Instance ltk_compat : Proper (eq ==> eq ==> iff) ltk.
+  Proof.
+    split; rewrite H, H0; trivial.
+  Qed.
+
+  
+  Global Instance ltk_compatk : Proper (eqk==>eqk==>iff) ltk.
+  Proof.
+  intros (x,e) (x',e') Hxx' (y,f) (y',f') Hyy'; compute.
+   compute in Hxx'; compute in Hyy'. rewrite Hxx', Hyy'; auto.
+  Qed.
+
+  Global Instance ltk_compat' : Proper (eqke==>eqke==>iff) ltk.
+  Proof.
+  intros (x,e) (x',e') (Hxx',_) (y,f) (y',f') (Hyy',_); compute.
+   compute in Hxx'; compute in Hyy'. rewrite Hxx', Hyy'; auto.
+  Qed.
+
+
+  Global Instance ltk_asym : Asymmetric ltk.
+  Proof. apply (StrictOrder_Asymmetric ltk_strorder). Qed.
+    
+
+  (* Additional facts *)
+
+  Lemma eqk_not_ltk : forall x x', eqk x x' -> ~ltk x x'.
+  Proof.
+    unfold eqk, ltk.
+    unfold not. intros x x' H.
+    destruct x, x'. simpl in *.
+    intro.
+    symmetry in H.
+    apply lt_not_eq in H. auto.
+    subst. auto.
+  Qed.
+
+  
+  Lemma ltk_eqk : forall e e' e'', ltk e e' -> eqk e' e'' -> ltk e e''.
+  Proof. unfold ltk, eqk. destruct e, e', e''. simpl.
+    intros; subst; trivial.
+  Qed.
+
+  Lemma eqk_ltk : forall e e' e'', eqk e e' -> ltk e' e'' -> ltk e e''.
+  Proof.
+    intros (k,e) (k',e') (k'',e'').
+    unfold ltk, eqk; simpl; intros; subst; trivial.
+  Qed.
+  Hint Resolve eqk_not_ltk.
+  Hint Immediate ltk_eqk eqk_ltk.
+  
   Lemma InA_eqke_eqk :
      forall x m, InA eqke x m -> InA eqk x m.
   Proof.
@@ -88,18 +317,26 @@ Section Array.
 
   Hint Resolve InA_eqke_eqk.
 
-  Lemma InA_eqk : forall p q m, eqk p q -> InA eqk p m -> InA eqk q m.
-  Proof.
-   intros; apply InA_eqA with p; auto with *.
-  Qed.
+  (* Lemma InA_eqk : forall p q m, eqk p q -> InA eqk p m -> InA eqk q m. *)
+  (* Proof. *)
+  (*  intros; apply InA_eqA with p; auto with *. *)
+  (* Qed. *)
 
+  (* Lemma In_eq : forall l x y, eq x y -> InA eqke x l -> InA eqke y l. *)
+  (* Proof. intros. rewrite <- H; auto. Qed. *)
 
+  (* Lemma ListIn_In : forall l x, List.In x l -> InA eqk x l. *)
+  (* Proof. apply In_InA. split; auto. unfold Transitive. *)
+  (*   unfold eqk; intros. rewrite H, <- H0. auto. *)
+  (* Qed. *)
   
-  Definition MapsTo (k:key)(e:elt):= InA eqke (k,e).
-  Definition In k m := exists e:elt, MapsTo k e m.
-  Notation NoDupA := (NoDupA eqk).
+  (* Lemma Inf_lt : forall l x y, ltk x y -> Inf y l -> Inf x l. *)
+  (* Proof. exact (InfA_ltA ltk_strorder). Qed. *)
 
-  Hint Unfold MapsTo In.
+  (* Lemma Inf_eq : forall l x y, x = y -> Inf y l -> Inf x l. *)
+  (* Proof. exact (InfA_eqA eq_equiv ltk_compat). Qed. *)
+
+
 
   (* An alternative formulation for [In k l] is [exists e, InA eqk (k,e) l] *)
 
@@ -114,17 +351,72 @@ Section Array.
   exists e; auto.
   Qed.
 
-  Lemma MapsTo_eq : forall l x y e, x = y -> MapsTo x e l -> MapsTo y e l.
+  Lemma MapsTo_eq : forall l x y e, eq x y -> MapsTo x e l -> MapsTo y e l.
   Proof.
   intros; unfold MapsTo in *; apply InA_eqA with (x,e); eauto with *.
   Qed.
 
-  Lemma In_eq : forall l x y, x = y -> In x l -> In y l.
+  Lemma In_eq : forall l x y, eq x y -> In x l -> In y l.
   Proof.
   destruct 2 as (e,E); exists e; eapply MapsTo_eq; eauto.
   Qed.
 
-  Lemma In_inv : forall k k' e l, In k ((k',e) :: l) -> k = k' \/ In k l.
+  Lemma Inf_eq : forall l x x', eqk x x' -> Inf x' l -> Inf x l.
+  Proof. exact (InfA_eqA eqk_equiv ltk_compatk). Qed.
+
+  Lemma Inf_lt : forall l x x', ltk x x' -> Inf x' l -> Inf x l.
+  Proof. exact (InfA_ltA ltk_strorder). Qed.
+
+  Hint Immediate Inf_eq.
+  Hint Resolve Inf_lt.
+
+  
+
+  Lemma Sort_Inf_In :
+    forall l p q, Sort l -> Inf q l -> InA eqk p l -> ltk q p.
+  Proof.
+    exact (SortA_InfA_InA eqk_equiv ltk_strorder ltk_compatk).
+  Qed.
+
+
+  
+  Lemma Sort_Inf_NotIn :
+    forall l k e, Sort l -> Inf (k,e) l ->  ~In k l.
+  Proof.
+    intros; red; intros.
+    destruct H1 as [e' H2].
+    elim (@ltk_not_eqk (k,e) (k,e')).
+    eapply Sort_Inf_In; eauto.
+    red; simpl; auto.
+  Qed.
+
+  Hint Resolve Sort_Inf_NotIn.
+  
+  Lemma Sort_NoDupA: forall l, Sort l -> NoDupA l.
+  Proof.
+    exact (SortA_NoDupA eqk_equiv ltk_strorder ltk_compatk).
+  Qed.
+
+  Lemma Sort_In_cons_1 : forall e l e', Sort (e::l) -> InA eqk e' l -> ltk e e'.
+  Proof.
+    inversion 1; intros; eapply Sort_Inf_In; eauto.
+  Qed.
+
+  Lemma Sort_In_cons_2 : forall l e e', Sort (e::l) -> InA eqk e' (e::l) ->
+                                   ltk e e' \/ eqk e e'.
+  Proof.
+    inversion_clear 2; auto.
+    left; apply Sort_In_cons_1 with l; auto.
+  Qed.
+
+  Lemma Sort_In_cons_3 :
+    forall x l k e, Sort ((k,e)::l) -> In x l -> ~eq x k.
+  Proof.
+    inversion_clear 1; red; intros.
+    destruct (Sort_Inf_NotIn H0 H1 (In_eq H2 H)).
+  Qed.
+
+  Lemma In_inv : forall k k' e l, In k ((k',e) :: l) -> eq k k' \/ In k l.
   Proof.
     inversion 1.
     inversion_clear H0; eauto.
@@ -134,22 +426,30 @@ Section Array.
   Lemma In_inv_2 : forall k k' e e' l,
       InA eqk (k, e) ((k', e') :: l) -> ~ eq k k' -> InA eqk (k, e) l.
   Proof.
-   inversion_clear 1; compute in H0; intuition.
+    inversion_clear 1; compute in H0; intuition.
   Qed.
 
   Lemma In_inv_3 : forall x x' l,
       InA eqke x (x' :: l) -> ~ eqk x x' -> InA eqke x l.
   Proof.
-   inversion_clear 1; compute in H0; intuition.
+    inversion_clear 1; compute in H0; intuition.
   Qed.
-
 
   Hint Resolve In_inv_2 In_inv_3.
 
 
+
+
+  (** * FMAPLIST interface implementaion  *)
+
+
+
+
+  (** * [empty] *)
+
   Definition empty : farray := nil.
 
-  Definition Empty m := forall (a : key)(e:elt), ~ MapsTo a e m.
+  Definition Empty m := forall (a : key)(e:elt) , ~ MapsTo a e m.
 
   Lemma empty_1 : Empty empty.
   Proof.
@@ -158,15 +458,13 @@ Section Array.
     intro abs.
     inversion abs.
   Qed.
-
   Hint Resolve empty_1.
 
-  Lemma empty_NoDup : NoDupA empty.
+  Lemma empty_sorted : Sort empty.
   Proof.
     unfold empty; auto.
   Qed.
 
-  
   (** * [is_empty] *)
 
   Definition is_empty (l : farray) : bool := if l then true else false.
@@ -176,9 +474,8 @@ Section Array.
     unfold Empty, MapsTo.
     intros m.
     case m;auto.
-    intros p l inlist.
-    destruct p.
-    absurd (InA eqke (k, e) ((k, e) :: l)); auto.
+    intros (k,e) l inlist.
+    absurd (InA eqke (k, e) ((k, e) :: l));auto.
   Qed.
 
   Lemma is_empty_2 : forall m, is_empty m = true -> Empty m.
@@ -194,31 +491,41 @@ Section Array.
   Function mem (k : key) (s : farray) {struct s} : bool :=
     match s with
     | nil => false
-    | (k',_) :: l => if eq_dec k k' then true else mem k l
+    | (k',_) :: l =>
+      match compare k k' with
+      | LT _ => false
+      | EQ _ => true
+      | GT _ => mem k l
+      end
     end.
 
-  Lemma mem_1 : forall m (Hm:NoDupA m) x, In x m -> mem x m = true.
+  Lemma mem_1 : forall m (Hm:Sort m) x, In x m -> mem x m = true.
   Proof.
     intros m Hm x; generalize Hm; clear Hm.
-    functional induction (mem x m);intros NoDup belong1;trivial.
+    functional induction (mem x m);intros sorted belong1;trivial.
+
     inversion belong1. inversion H.
-    inversion_clear NoDup.
-    inversion_clear belong1.
-    inversion_clear H1.
-    compute in H2; destruct H2.
-    contradiction.
-    apply IHb; auto.
-    exists x0; auto.
+
+    absurd (In x ((k', _x) :: l));try assumption.
+    apply Sort_Inf_NotIn with _x;auto.
+
+    apply IHb.
+    elim (sort_inv sorted);auto.
+    elim (In_inv belong1);auto.
+    intro abs.
+    absurd (eq x k'); auto.
+    symmetry in abs.
+    apply lt_not_eq in abs; auto.
   Qed.
 
-  Lemma mem_2 : forall m (Hm:NoDupA m) x, mem x m = true -> In x m.
+  Lemma mem_2 : forall m (Hm:Sort m) x, mem x m = true -> In x m.
   Proof.
     intros m Hm x; generalize Hm; clear Hm; unfold In,MapsTo.
-    functional induction (mem x m); intros NoDup hyp; try discriminate.
+    functional induction (mem x m); intros sorted hyp;try ((inversion hyp);fail).
     exists _x; auto.
-    inversion_clear NoDup.
-    destruct IHb; auto.
+    induction IHb; auto.
     exists x0; auto.
+    inversion_clear sorted; auto.
   Qed.
 
   (** * [find] *)
@@ -226,42 +533,49 @@ Section Array.
   Function find (k:key) (s: farray) {struct s} : option elt :=
     match s with
     | nil => None
-    | (k',x)::s' => if eq_dec k k' then Some x else find k s'
+    | (k',x)::s' =>
+      match compare k k' with
+      | LT _ => None
+      | EQ _ => Some x
+      | GT _ => find k s'
+      end
     end.
 
-  Lemma find_2 : forall m x e, find x m = Some e -> MapsTo x e m.
+  Lemma find_2 :  forall m x e, find x m = Some e -> MapsTo x e m.
   Proof.
     intros m x. unfold MapsTo.
     functional induction (find x m);simpl;intros e' eqfind; inversion eqfind; auto.
   Qed.
 
-  Lemma find_1 : forall m (Hm:NoDupA m) x e,
-      MapsTo x e m -> find x m = Some e.
+  Lemma find_1 :  forall m (Hm:Sort m) x e, MapsTo x e m -> find x m = Some e.
   Proof.
     intros m Hm x e; generalize Hm; clear Hm; unfold MapsTo.
     functional induction (find x m);simpl; subst; try clear H_eq_1.
 
     inversion 2.
 
-    do 2 inversion_clear 1.
-    compute in H2; destruct H2; subst; trivial.
-    elim H; apply InA_eqk with (x,e); auto.
+    inversion_clear 2.
+    clear e1;compute in H0; destruct H0.
+    apply lt_not_eq in H; auto. now contradict H.
 
-    do 2 inversion_clear 1; auto.
-    compute in H2; destruct H2; elim _x; auto.
-  Qed.
-
-  (* Not part of the exported specifications, used later for [combine]. *)
-
-  Lemma find_eq : forall m (Hm:NoDupA m) x x',
-      eq x x' -> find x m = find x' m.
-  Proof.
-    induction m; simpl; auto; destruct a; intros.
-    inversion_clear Hm.
-    rewrite (IHm H1 x x'); auto.
-    destruct (eq_dec x k); destruct (eq_dec x' k); trivial.
-    elim n; apply eq_trans with x; auto.
-    elim n; apply eq_trans with x'; auto.
+    clear e1;generalize (Sort_In_cons_1 Hm (InA_eqke_eqk H0)); compute.
+    (* order. *)
+    intros.
+    apply (lt_trans k') in _x; auto.
+    apply lt_not_eq in _x.
+    now contradict _x.
+    
+    clear e1;inversion_clear 2.
+    compute in H0; destruct H0; intuition congruence.
+    generalize (Sort_In_cons_1 Hm (InA_eqke_eqk H0)); compute.
+    (* order. *)
+    intros.
+    apply lt_not_eq in H. now contradict H.
+    
+    clear e1; do 2 inversion_clear 1; auto.
+    compute in H2; destruct H2.
+    (* order. *)
+    subst. apply lt_not_eq in _x. now contradict _x.
   Qed.
 
   (** * [add] *)
@@ -269,404 +583,704 @@ Section Array.
   Function add (k : key) (x : elt) (s : farray) {struct s} : farray :=
     match s with
     | nil => (k,x) :: nil
-    | (k',y) :: l => if eq_dec k k' then (k,x)::l else (k',y)::add k x l
+    | (k',y) :: l =>
+      match compare k k' with
+      | LT _ => (k,x)::s
+      | EQ _ => (k,x)::l
+      | GT _ => (k',y) :: add k x l
+      end
     end.
 
   Lemma add_1 : forall m x y e, eq x y -> MapsTo y e (add x e m).
   Proof.
-    intros m x y e; generalize y; clear y; unfold MapsTo.
+    intros m x y e; generalize y; clear y.
+    unfold MapsTo.
     functional induction (add x e m);simpl;auto.
   Qed.
 
   Lemma add_2 : forall m x y e e',
       ~ eq x y -> MapsTo y e m -> MapsTo y e (add x e' m).
   Proof.
-    intros m x  y e e'; generalize y e; clear y e; unfold MapsTo.
-    functional induction (add x e' m);simpl;auto.
-    intros y' e'' eqky';  inversion_clear 1.
-    destruct H0; simpl in *.
-    elim eqky'; auto.
+    intros m x  y e e'.
+    generalize y e; clear y e; unfold MapsTo.
+    functional induction (add x e' m) ;simpl;auto;  clear e0.
+    subst;auto.
+
+    intros y' e'' eqky';  inversion_clear 1;  destruct H0; simpl in *.
+    (* order. *)
+    subst. now contradict eqky'.
+    auto.
     auto.
     intros y' e'' eqky'; inversion_clear 1; intuition.
   Qed.
+
 
   Lemma add_3 : forall m x y e e',
       ~ eq x y -> MapsTo y e (add x e' m) -> MapsTo y e m.
   Proof.
     intros m x y e e'. generalize y e; clear y e; unfold MapsTo.
-    functional induction (add x e' m);simpl;auto.
-    intros; eauto.
-    constructor 2; eauto.
-    inversion_clear 2; auto.
+    functional induction (add x e' m);simpl; intros.
+    apply (In_inv_3 H0); compute; auto.
+    apply (In_inv_3 H0); compute; auto.
+    constructor 2; apply (In_inv_3 H0); compute; auto.
+    inversion_clear H0; auto.
   Qed.
 
-  Lemma add_3' : forall m x y e e',
-      ~ eq x y -> InA eqk (y,e) (add x e' m) -> InA eqk (y,e) m.
-  Proof.
-    intros m x y e e'. generalize y e; clear y e.
-    functional induction (add x e' m);simpl;auto.
-    inversion_clear 2.
-    compute in H1; elim H; auto.
-    inversion H1.
-    constructor 2; inversion_clear H0; auto.
-    compute in H1; elim H; auto.
-    inversion_clear 2; auto.
-  Qed.
 
-  Lemma add_NoDup : forall m (Hm:NoDupA m) x e, NoDupA (add x e m).
+  Lemma add_Inf : forall (m:farray)(x x':key)(e e':elt),
+      Inf (x',e') m -> ltk (x',e') (x,e) -> Inf (x',e') (add x e m).
   Proof.
     induction m.
-    simpl; constructor; auto; red; inversion 1.
+    simpl; intuition.
+    intros.
+    destruct a as (x'',e'').
+    inversion_clear H.
+    compute in H0,H1.
+    simpl; case (compare x x''); intuition.
+  Qed.
+  Hint Resolve add_Inf.
+
+  Lemma add_sorted : forall m (Hm:Sort m) x e, Sort (add x e m).
+  Proof.
+    induction m.
+    simpl; intuition.
     intros.
     destruct a as (x',e').
-    simpl; case (eq_dec x x'); inversion_clear Hm; auto.
+    simpl; case (compare x x'); intuition; inversion_clear Hm; auto.
     constructor; auto.
-    contradict H.
-    apply InA_eqk with (x,e); auto.
-    constructor; auto.
-    contradict H; apply add_3' with x e; auto.
+    apply Inf_eq with (x',e'); auto.
   Qed.
-
-  (* Not part of the exported specifications, used later for [combine]. *)
-
-  Lemma add_eq : forall m (Hm:NoDupA m) x a e,
-      eq x a -> find x (add a e m) = Some e.
-  Proof.
-    intros.
-    apply find_1; auto.
-    apply add_NoDup; auto.
-    apply add_1; auto.
-  Qed.
-
-  Lemma add_not_eq : forall m (Hm:NoDupA m) x a e,
-      ~eq x a -> find x (add a e m) = find x m.
-  Proof.
-    intros.
-    case_eq (find x m); intros.
-    apply find_1; auto.
-    apply add_NoDup; auto.
-    apply add_2; auto.
-    apply find_2; auto.
-    case_eq (find x (add a e m)); intros; auto.
-    rewrite <- H0; symmetry.
-    apply find_1; auto.
-    apply add_3 with a e; auto.
-    apply find_2; auto.
-  Qed.
-
-
 
   (** * [remove] *)
 
   Function remove (k : key) (s : farray) {struct s} : farray :=
     match s with
     | nil => nil
-    | (k',x) :: l => if eq_dec k k' then l else (k',x) :: remove k l
+    | (k',x) :: l =>
+      match compare k k' with
+      | LT _ => s
+      | EQ _ => l
+      | GT _ => (k',x) :: remove k l
+      end
     end.
 
-  Lemma remove_1 : forall m (Hm:NoDupA m) x y, x = y -> ~ In y (remove x m).
+  Lemma remove_1 : forall m (Hm:Sort m) x y, eq x y -> ~ In y (remove x m).
   Proof.
     intros m Hm x y; generalize Hm; clear Hm.
-    functional induction (remove x m);simpl;intros;auto.
+    functional induction (remove x m);simpl;intros;subst.
 
-    red; inversion 1; inversion H1.
+    red; inversion 1; inversion H0.
 
-    inversion_clear Hm.
-    subst.
-    contradict H0.
-    destruct H0 as (e,H2); unfold MapsTo in H2.
-    apply InA_eqk with (y,e); auto.
-    compute; auto.
+    apply Sort_Inf_NotIn with x0; auto.
 
-    intro H2.
-    destruct H2 as (e,H2); inversion_clear H2.
-    compute in H0; destruct H0.
-    elim _x; apply eq_trans with y; auto.
-    inversion_clear Hm.
-    elim (IHf H2 H).
-    exists e; auto.
+    clear e0. inversion Hm. subst.
+    apply Sort_Inf_NotIn with x0; auto.
+    
+
+    (* clear e0;inversion_clear Hm. *)
+    (* apply Sort_Inf_NotIn with x0; auto. *)
+    (* apply Inf_eq with (k',x0);auto; compute; apply eq_trans with x; auto. *)
+
+    clear e0;inversion_clear Hm.
+    assert (notin:~ In y (remove y l)) by auto.
+    intros (x1,abs).
+    inversion_clear abs.
+    compute in H1; destruct H1.
+    subst. apply lt_not_eq in _x; now contradict _x.
+    apply notin; exists x1; auto.
   Qed.
 
-  Lemma remove_2 : forall m (Hm:NoDupA m) x y e,
-      x <> y -> MapsTo y e m -> MapsTo y e (remove x m).
+
+  Lemma remove_2 : forall m (Hm:Sort m) x y e,
+      ~ eq x y -> MapsTo y e m -> MapsTo y e (remove x m).
   Proof.
     intros m Hm x y e; generalize Hm; clear Hm; unfold MapsTo.
-    functional induction (remove x m);auto.
+    functional induction (remove x m);subst;auto;
+      match goal with
+      | [H: compare _ _ = _ |- _ ] => clear H
+      | _ => idtac
+      end.
+
     inversion_clear 3; auto.
     compute in H1; destruct H1.
-    elim H; auto.
-
+    subst; now contradict H.
     inversion_clear 1; inversion_clear 2; auto.
   Qed.
 
-  Lemma remove_3 : forall m (Hm:NoDupA m) x y e,
+  Lemma remove_3 : forall m (Hm:Sort m) x y e,
       MapsTo y e (remove x m) -> MapsTo y e m.
   Proof.
     intros m Hm x y e; generalize Hm; clear Hm; unfold MapsTo.
-    functional induction (remove x m);auto.
-    do 2 inversion_clear 1; auto.
+    functional induction (remove x m);subst;auto.
+    inversion_clear 1; inversion_clear 1; auto.
   Qed.
 
-  Lemma remove_3' : forall m (Hm:NoDupA m) x y e,
-      InA eqk (y,e) (remove x m) -> InA eqk (y,e) m.
-  Proof.
-    intros m Hm x y e; generalize Hm; clear Hm; unfold MapsTo.
-    functional induction (remove x m);auto.
-    do 2 inversion_clear 1; auto.
-  Qed.
-
-  Lemma remove_NoDup : forall m (Hm:NoDupA m) x, NoDupA (remove x m).
+  Lemma remove_Inf : forall (m:farray)(Hm : Sort m)(x x':key)(e':elt),
+      Inf (x',e') m -> Inf (x',e') (remove x m).
   Proof.
     induction m.
     simpl; intuition.
     intros.
+    destruct a as (x'',e'').
+    inversion_clear H.
+    compute in H0.
+    simpl; case (compare x x''); intuition.
     inversion_clear Hm.
+    apply Inf_lt with (x'',e''); auto.
+  Qed.
+  Hint Resolve remove_Inf.
+
+  Lemma remove_sorted : forall m (Hm:Sort m) x, Sort (remove x m).
+  Proof.
+    induction m.
+    simpl; intuition.
+    intros.
     destruct a as (x',e').
-    simpl; case (eq_dec x x'); auto.
-    constructor; auto.
-    contradict H; apply remove_3' with x; auto.
+    simpl; case (compare x x'); intuition; inversion_clear Hm; auto.
   Qed.
 
-  
   (** * [elements] *)
 
   Definition elements (m: farray) := m.
 
-  Lemma elements_1 : forall m x e, MapsTo x e m -> InA eqke (x,e) (elements m).
+  Lemma elements_1 : forall m x e,
+      MapsTo x e m -> InA eqke (x,e) (elements m).
   Proof.
     auto.
   Qed.
 
-  Lemma elements_2 : forall m x e, InA eqke (x,e) (elements m) -> MapsTo x e m.
+  Lemma elements_2 : forall m x e,
+      InA eqke (x,e) (elements m) -> MapsTo x e m.
   Proof.
     auto.
   Qed.
 
-  Lemma elements_3w : forall m (Hm:NoDupA m), NoDupA (elements m).
+  Lemma elements_3 : forall m (Hm:Sort m), sort ltk (elements m).
   Proof.
     auto.
   Qed.
 
-  
+  Lemma elements_3w : forall m (Hm:Sort m), NoDupA (elements m).
+  Proof.
+    intros.
+    apply Sort_NoDupA.
+    apply elements_3; auto.
+  Qed.
+
   (** * [fold] *)
 
-  Function fold {A:Type} (f:key->elt->A->A) (m:farray) (acc : A) {struct m} :  A :=
+  Function fold (A:Type)(f:key->elt->A->A)(m:farray) (acc:A) {struct m} :  A :=
     match m with
     | nil => acc
     | (k,e)::m' => fold f m' (f k e acc)
     end.
 
-  Lemma fold_1 : forall m (A:Type) (i:A) (f:key->elt->A->A),
+  Lemma fold_1 : forall m (A:Type)(i:A)(f:key->elt->A->A),
       fold f m i = fold_left (fun a p => f (fst p) (snd p) a) (elements m) i.
   Proof.
-    intros; functional induction (@fold A f m i); auto.
+    intros; functional induction (fold f m i); auto.
   Qed.
 
-  
   (** * [equal] *)
 
-  Definition check (k:key)(e:elt)(m': farray) :=
-    match find k m' with
-    | None => false
-    | Some e' => eqb_elt e e'
+  Function equal (cmp:elt->elt->bool)(m m' : farray) {struct m} : bool :=
+    match m, m' with
+    | nil, nil => true
+    | (x,e)::l, (x',e')::l' =>
+      match compare x x' with
+      | EQ _ => cmp e e' && equal cmp l l'
+      | _    => false
+      end
+    | _, _ => false
     end.
 
-  Definition submap (m m' : farray) : bool :=
-    fold (fun k e b => andb (check k e m') b) m true.
-
-  Definition equal (m m' : farray) : bool :=
-    andb (submap m m') (submap m' m).
-
-  Definition Submap m m' :=
-    (forall k, In k m -> In k m') /\
-    (forall k e e', MapsTo k e m -> MapsTo k e' m' -> eqb_elt e e' = true).
-
-  Definition Equivb m m' :=
+  Definition Equivb cmp m m' :=
     (forall k, In k m <-> In k m') /\
-    (forall k e e', MapsTo k e m -> MapsTo k e' m' -> eqb_elt e e' = true).
+    (forall k e e', MapsTo k e m -> MapsTo k e' m' -> cmp e e' = true).
 
-  Lemma submap_1 : forall m (Hm:NoDupA m) m' (Hm': NoDupA m'),
-      Submap m m' -> submap m m' = true.
+  Lemma equal_1 : forall m (Hm:Sort m) m' (Hm': Sort m') cmp,
+      Equivb cmp m m' -> equal cmp m m' = true.
   Proof.
-    unfold Submap, submap.
-    induction m.
-    simpl; auto.
-    destruct a; simpl; intros.
-    destruct H.
+    intros m Hm m' Hm' cmp; generalize Hm Hm'; clear Hm Hm'.
+    functional induction (equal cmp m m'); simpl; subst;auto; unfold Equivb;
+      intuition; subst.
+    match goal with H: compare _ _ = _ |- _ => clear H end.
+    assert (cmp_e_e':cmp e e' = true).
+    apply H1 with x; auto.
+    rewrite cmp_e_e'; simpl.
+    apply IHb; auto.
+    inversion_clear Hm; auto.
+    inversion_clear Hm'; auto.
+    unfold Equivb; intuition.
+    destruct (H0 k).
+    assert (In k ((x,e) ::l)).
+    destruct H as (e'', hyp); exists e''; auto.
+    destruct (In_inv (H2 H4)); auto.
     inversion_clear Hm.
-    assert (H3 : In k m').
-    apply H; exists e; auto.
-    destruct H3 as (e', H3).
-    unfold check at 2; rewrite (find_1 Hm' H3).
-    rewrite (H0 k); simpl; auto.
-    eapply IHm; auto.
-    split; intuition.
-    apply H.
-    destruct H5 as (e'',H5); exists e''; auto.
-    apply (H0 k0); auto.
+    elim (Sort_Inf_NotIn H6 H7).
+    destruct H as (e'', hyp); exists e''; auto.
+    apply MapsTo_eq with k; auto.
+    destruct (H0 k).
+    assert (In k ((x,e') ::l')).
+    destruct H as (e'', hyp); exists e''; auto.
+    destruct (In_inv (H3 H4)); auto.
+    subst.
+    inversion_clear Hm'.
+    now elim (Sort_Inf_NotIn H5 H6).
+    apply H1 with k; destruct (eq_dec x k); auto.
+
+
+    destruct (compare x x') as [Hlt|Heq|Hlt]; try contradiction; clear y.
+    destruct (H0 x).
+    assert (In x ((x',e')::l')).
+    apply H; auto.
+    exists e; auto.
+    destruct (In_inv H3).
+    (* order. *)
+    apply lt_not_eq in Hlt; now contradict Hlt.
+    inversion_clear Hm'.
+    assert (Inf (x,e) l').
+    apply Inf_lt with (x',e'); auto.
+    elim (Sort_Inf_NotIn H5 H7 H4).
+
+    destruct (H0 x').
+    assert (In x' ((x,e)::l)).
+    apply H2; auto.
+    exists e'; auto.
+    destruct (In_inv H3).
+    (* order. *)
+    subst; apply lt_not_eq in Hlt; now contradict Hlt.
+    inversion_clear Hm.
+    assert (Inf (x',e') l).
+    apply Inf_lt with (x,e); auto.
+    elim (Sort_Inf_NotIn H5 H7 H4).
+
+    destruct m;
+      destruct m';try contradiction.
+
+    clear H1;destruct p as (k,e).
+    destruct (H0 k).
+    destruct H1.
+    exists e; auto.
+    inversion H1.
+
+    destruct p as (x,e).
+    destruct (H0 x).
+    destruct H.
+    exists e; auto.
+    inversion H.
+
+    destruct p;destruct p0;contradiction.
   Qed.
 
-  Lemma submap_2 : forall m (Hm:NoDupA m) m' (Hm': NoDupA m'),
-      submap m m' = true -> Submap m m'.
+
+  Lemma equal_2 : forall m (Hm:Sort m) m' (Hm:Sort m') cmp,
+      equal cmp m m' = true -> Equivb cmp m m'.
   Proof.
-    unfold Submap, submap.
-    induction m.
-    simpl; auto.
-    intuition.
-    destruct H0; inversion H0.
+    intros m Hm m' Hm' cmp; generalize Hm Hm'; clear Hm Hm'.
+    functional induction (equal cmp m m'); simpl; subst;auto; unfold Equivb;
+      intuition; try discriminate; subst;
+        try match goal with H: compare _ _ = _ |- _ => clear H end.
+
     inversion H0.
 
-    destruct a; simpl; intros.
-    inversion_clear Hm.
-    rewrite andb_b_true in H.
-    assert (check k e m' = true).
-    clear H1 H0 Hm' IHm.
-    set (b:=check k e m') in *.
-    generalize H; clear H; generalize b; clear b.
-    induction m; simpl; auto; intros.
-    destruct a; simpl in *.
-    destruct (andb_prop _ _ (IHm _ H)); auto.
-    rewrite H2 in H.
-    destruct (IHm H1 m' Hm' H); auto.
-    unfold check in H2.
-    case_eq (find k m'); [intros e' H5 | intros H5];
-      rewrite H5 in H2; try discriminate.
-    split; intros.
-    destruct H6 as (e0,H6); inversion_clear H6.
-    compute in H7; destruct H7; subst.
-    exists e'.
-    apply MapsTo_eq with k; auto.
-    apply find_2; auto.
-    apply H3.
-    exists e0; auto.
-    inversion_clear H6.
-    compute in H8; destruct H8; subst e0.
-    rewrite (find_1 Hm' (MapsTo_eq H6 H7)) in H5; congruence.
-    apply H4 with k0; auto.
-  Qed.
-
-  
-  (** Specification of [equal] *)
-
-  Lemma equal_1 : forall m (Hm:NoDupA m) m' (Hm': NoDupA m'),
-      Equivb m m' -> equal m m' = true.
-  Proof.
-    unfold Equivb, equal.
-    intuition.
-    apply andb_true_intro; split; apply submap_1; unfold Submap; firstorder.
-    apply eqb_elt_eq. symmetry. apply eqb_elt_eq. 
-    apply (H1 k e' e); auto.
-  Qed.
-
-  Lemma equal_2 : forall m (Hm:NoDupA m) m' (Hm':NoDupA m'),
-      equal m m' = true -> Equivb m m'.
-  Proof.
-    unfold Equivb, equal.
-    intros.
+    inversion_clear Hm;inversion_clear Hm'.
     destruct (andb_prop _ _ H); clear H.
-    generalize (submap_2 Hm Hm' H0).
-    generalize (submap_2 Hm' Hm H1).
-    firstorder.
+    destruct (IHb H1 H3 H6).
+    destruct (In_inv H0).
+    exists e'; constructor; split; trivial; apply eq_trans with x; auto.
+    destruct (H k).
+    destruct (H9 H8) as (e'',hyp).
+    exists e''; auto.
+
+    inversion_clear Hm;inversion_clear Hm'.
+    destruct (andb_prop _ _ H); clear H.
+    destruct (IHb H1 H3 H6).
+    destruct (In_inv H0).
+    exists e; constructor; split; trivial; apply eq_trans with x'; auto.
+    destruct (H k).
+    destruct (H10 H8) as (e'',hyp).
+    exists e''; auto.
+
+    inversion_clear Hm;inversion_clear Hm'.
+    destruct (andb_prop _ _ H); clear H.
+    destruct (IHb H2 H4 H7).
+    inversion_clear H0.
+    destruct H9; simpl in *; subst.
+    inversion_clear H1.
+    destruct H0; simpl in *; subst; auto.
+    elim (Sort_Inf_NotIn H4 H5).
+    exists e'0; apply MapsTo_eq with x; auto.
+      (* order. *)
+    inversion_clear H1.
+    destruct H0; simpl in *; subst; auto.
+    elim (Sort_Inf_NotIn H2 H3).
+    exists e0; apply MapsTo_eq with x; auto.
+    (* order. *)
+    apply H8 with k; auto.
   Qed.
 
+  (** This lemma isn't part of the spec of [Equivb], but is used in [FMapAVL] *)
+
+  Lemma equal_cons : forall cmp l1 l2 x y, Sort (x::l1) -> Sort (y::l2) ->
+    eqk x y -> cmp (snd x) (snd y) = true ->
+    (Equivb cmp l1 l2 <-> Equivb cmp (x :: l1) (y :: l2)).
+  Proof.
+    intros.
+    inversion H; subst.
+    inversion H0; subst.
+    destruct x; destruct y; compute in H1, H2.
+    split; intros.
+    apply equal_2; auto.
+    simpl.
+    case (compare k k0);
+    subst; intro HH; try (apply lt_not_eq in HH; now contradict HH).
+    rewrite H2; simpl.
+    apply equal_1; auto.
+    apply equal_2; auto.
+    generalize (equal_1 H H0 H3).
+    simpl.
+    case (compare k k0);
+    subst; intro HH; try (apply lt_not_eq in HH; now contradict HH).
+    rewrite H2; simpl; auto.
+  Qed.
+
+End Array.
+
+End Raw.
 
 
 
+Section FArray.
+
+  Variable key : Type.
+  Variable elt : Type.
+  Variable key_dec : DecType key.
+  Variable key_ord : OrdType key.
+  Variable key_comp : Comparable key.
+  Variable elt_dec : DecType elt.
+  Variable elt_ord : OrdType elt.
+  Variable elt_comp : Comparable elt.
+
+  Set Implicit Arguments.
 
   Record slist :=
-    {this :> farray; NoDup : NoDupA this}.
-  Definition _farray := slist.
+    {this :> Raw.farray key elt; sorted : sort (Raw.ltk key_ord) this}.
+  Definition farray := slist.
 
-  (* Definition _MapsTo (k:key)(e:elt) m := InA eqke (k,e) m.(this). *)
-  (* Definition _In k m := exists e:elt, _MapsTo k e m. *)
-
-  (* Definition _MapsTo (k:key)(e:elt) m := MapsTo k e m.(this). *)
-  (* Definition _In k m := In k m.(this). *)
-
-  Definition _empty : _farray := Build_slist empty_NoDup.
-  Definition _is_empty m : bool := is_empty m.(this).
-  Definition _add x e m : _farray := Build_slist (add_NoDup m.(NoDup) x e).
-  Definition _find x m : option elt := find x m.(this).
-  Definition _remove x m : _farray := Build_slist (remove_NoDup m.(NoDup) x).
-  Definition _mem x m : bool := mem x m.(this).
-  (* Definition _map f m : _farray := Build_slist (map_NoDup m.(NoDup) f). *)
-  (* Definition _mapi (f:key->elt->elt') m : _farray' := Build_slist (mapi_NoDup m.(NoDup) f). *)
-  (* Definition _map2 f m (m':_farray') : _farray'' := *)
-  (*   Build_slist (map2_NoDup f m.(NoDup) m'.(NoDup)). *)
-  Definition _elements m : list (key*elt) := @elements m.(this).
-  Definition _cardinal m := length m.(this).
-  Definition _fold (A:Type)(f:key->elt->A->A) m (i:A) : A := @fold A f m.(this) i.
-  Definition _equal m m' : bool := @equal m.(this) m'.(this).
-  Definition _MapsTo x e m : Prop := MapsTo x e m.(this).
-  Definition _In x m : Prop := In x m.(this).
-  Definition _Empty m : Prop := Empty m.(this).
-
-  Definition _Equal m m' := forall y, _find y m = _find y m'.
-  Definition _Equiv m m' :=
-    (forall k, _In k m <-> _In k m') /\
-    (forall k e e', _MapsTo k e m -> _MapsTo k e' m' -> e = e').
-  Definition _Equivb m m' : Prop := @Equivb m.(this) m'.(this).
-
-  Definition _eq_key : (key*elt) -> (key*elt) -> Prop := eqk.
-  Definition _eq_key_elt : (key*elt) -> (key*elt) -> Prop:= @eqke.
-
-  Lemma MapsTo_1 : forall m x y e, x = y -> _MapsTo x e m -> _MapsTo y e m.
-  Proof. intros m; exact (@MapsTo_eq m.(this)). Qed.
-
-  Lemma _mem_1 : forall m x, _In x m -> _mem x m = true.
-  Proof. intros m; exact (@mem_1 m.(this) m.(NoDup)). Qed.
+  (* Boolean comparison over elements *)
+  Definition cmp (e e':elt) :=
+    match compare e e' with EQ _ => true | _ => false end.
   
-  Lemma _mem_2 : forall m x, _mem x m = true -> _In x m.
-  Proof. intros m; exact (@mem_2 m.(this) m.(NoDup)). Qed.
+  Definition empty : farray := Build_slist (Raw.empty_sorted elt key_ord).
+  Definition is_empty m : bool := Raw.is_empty m.(this).
+  Definition add x e m : farray :=
+    Build_slist (Raw.add_sorted key_dec key_comp m.(sorted) x e).
+  Definition find x m : option elt := Raw.find key_comp x m.(this).
+  Definition remove x m : farray :=
+    Build_slist (Raw.remove_sorted key_comp m.(sorted) x).
+  Definition mem x m : bool := Raw.mem key_comp x m.(this).
+  Definition elements m : list (key*elt) := Raw.elements m.(this).
+  Definition cardinal m := length m.(this).
+  Definition fold (A:Type)(f:key->elt->A->A) m (i:A) : A :=
+    Raw.fold f m.(this) i.
+  Definition equal m m' : bool := Raw.equal key_comp cmp m.(this) m'.(this).
 
-  Lemma _empty_1 : _Empty _empty.
-  Proof. exact (@empty_1). Qed.
+  Definition MapsTo x e m : Prop := Raw.MapsTo x e m.(this).
+  Definition In x m : Prop := Raw.In x m.(this).
+  Definition Empty m : Prop := Raw.Empty m.(this).
 
-  Lemma _is_empty_1 : forall m, _Empty m -> _is_empty m = true.
-  Proof. intros m; exact (@is_empty_1 m.(this)). Qed.
-  Lemma _is_empty_2 :  forall m, _is_empty m = true -> _Empty m.
-  Proof. intros m; exact (@is_empty_2 m.(this)). Qed.
+  Definition Equal m m' := forall y, find y m = find y m'.
+  Definition Equiv m m' :=
+    (forall k, In k m <-> In k m') /\
+    (forall k e e', MapsTo k e m -> MapsTo k e' m' -> e = e').
+  Definition Equivb m m' : Prop := Raw.Equivb cmp m.(this) m'.(this).
 
-  Lemma _add_1 : forall m x y e, x = y -> _MapsTo y e (_add x e m).
-  Proof. intros m; exact (@add_1 m.(this)). Qed.
-  
-  Lemma _add_2 : forall m x y e e', x <> y -> _MapsTo y e m -> _MapsTo y e (_add x e' m).
-  Proof. intros m; exact (@add_2 m.(this)). Qed.
-  
-  Lemma _add_3 : forall m x y e e', x <> y -> _MapsTo y e (_add x e' m) -> _MapsTo y e m.
-  Proof. intros m; exact (@add_3 m.(this)). Qed.
+  Definition eq_key : (key*elt) -> (key*elt) -> Prop := @Raw.eqk key elt.
+  Definition eq_key_elt : (key*elt) -> (key*elt) -> Prop:= @Raw.eqke key elt.
+  Definition lt_key : (key*elt) -> (key*elt) -> Prop := @Raw.ltk key elt key_ord.
 
-  Lemma _remove_1 : forall m x y, x = y -> ~ _In y (_remove x m).
-  Proof. intros m; exact (@remove_1 m.(this) m.(NoDup)). Qed.
-  
-  Lemma _remove_2 : forall m x y e, x <> y -> _MapsTo y e m -> _MapsTo y e (_remove x m).
-  Proof. intros m; exact (@remove_2 m.(this) m.(NoDup)). Qed.
-  Lemma _remove_3 : forall m x y e, _MapsTo y e (_remove x m) -> _MapsTo y e m.
-  Proof. intros m; exact (@remove_3 m.(this) m.(NoDup)). Qed.
+  Lemma MapsTo_1 : forall m x y e, eq x y -> MapsTo x e m -> MapsTo y e m.
+  Proof. intros m.
+    apply (Raw.MapsTo_eq key_dec elt_dec). Qed.
 
-  Lemma _find_1 : forall m x e, _MapsTo x e m -> _find x m = Some e.
-  Proof. intros m; exact (@find_1 m.(this) m.(NoDup)). Qed.
-  Lemma _find_2 : forall m x e, _find x m = Some e -> _MapsTo x e m.
-  Proof. intros m; exact (@find_2 m.(this)). Qed.
+  Lemma mem_1 : forall m x, In x m -> mem x m = true.
+  Proof. intros m; apply (Raw.mem_1); auto. apply m.(sorted). Qed.
+  Lemma mem_2 : forall m x, mem x m = true -> In x m.
+  Proof. intros m; apply (Raw.mem_2); auto. apply m.(sorted). Qed.
 
-  Lemma _elements_1 : forall m x e, _MapsTo x e m -> InA eqke (x,e) (_elements m).
-  Proof. intros m; exact (@elements_1 m.(this)). Qed.
-  Lemma _elements_2 : forall m x e, InA eqke (x,e) (_elements m) -> _MapsTo x e m.
-  Proof. intros m; exact (@elements_2 m.(this)). Qed.
-  Lemma _elements_3w : forall m, NoDupA (_elements m).
-  Proof. intros m; exact (@elements_3w m.(this) m.(NoDup)). Qed.
+  Lemma empty_1 : Empty empty.
+  Proof. apply Raw.empty_1. Qed.
 
-  Lemma _cardinal_1 : forall m, _cardinal m = length (_elements m).
+  Lemma is_empty_1 : forall m, Empty m -> is_empty m = true.
+  Proof. intros m; apply Raw.is_empty_1. Qed.
+  Lemma is_empty_2 :  forall m, is_empty m = true -> Empty m.
+  Proof. intros m; apply Raw.is_empty_2. Qed.
+
+  Lemma add_1 : forall m x y e, eq x y -> MapsTo y e (add x e m).
+  Proof. intros m; apply Raw.add_1; auto. Qed.
+  Lemma add_2 : forall m x y e e', ~ eq x y -> MapsTo y e m -> MapsTo y e (add x e' m).
+  Proof. intros m; apply Raw.add_2; auto. Qed.
+  Lemma add_3 : forall m x y e e', ~ eq x y -> MapsTo y e (add x e' m) -> MapsTo y e m.
+  Proof. intros m; apply Raw.add_3; auto. Qed.
+
+  Lemma remove_1 : forall m x y, eq x y -> ~ In y (remove x m).
+  Proof. intros m; apply Raw.remove_1; auto. apply m.(sorted). Qed.
+  Lemma remove_2 : forall m x y e, ~ eq x y -> MapsTo y e m -> MapsTo y e (remove x m).
+  Proof. intros m; apply Raw.remove_2; auto. apply m.(sorted). Qed.
+  Lemma remove_3 : forall m x y e, MapsTo y e (remove x m) -> MapsTo y e m.
+  Proof. intros m; apply Raw.remove_3; auto. apply m.(sorted). Qed.
+
+  Lemma find_1 : forall m x e, MapsTo x e m -> find x m = Some e.
+  Proof. intros m; apply Raw.find_1; auto. apply m.(sorted). Qed.
+  Lemma find_2 : forall m x e, find x m = Some e -> MapsTo x e m.
+  Proof. intros m; apply Raw.find_2; auto. Qed.
+
+  Lemma elements_1 : forall m x e, MapsTo x e m -> InA eq_key_elt (x,e) (elements m).
+  Proof. intros m; apply Raw.elements_1. Qed.
+  Lemma elements_2 : forall m x e, InA eq_key_elt (x,e) (elements m) -> MapsTo x e m.
+  Proof. intros m; apply Raw.elements_2. Qed.
+  Lemma elements_3 : forall m, sort lt_key (elements m).
+  Proof. intros m; apply Raw.elements_3; auto. apply m.(sorted). Qed.
+  Lemma elements_3w : forall m, NoDupA eq_key (elements m).
+  Proof. intros m; apply (Raw.elements_3w key_dec m.(sorted)). Qed.
+
+  Lemma cardinal_1 : forall m, cardinal m = length (elements m).
   Proof. intros; reflexivity. Qed.
 
-  Lemma _fold_1 : forall m (A : Type) (i : A) (f : key -> elt -> A -> A),
-      _fold f m i = fold_left (fun a p => f (fst p) (snd p) a) (_elements m) i.
-  Proof. intros m; exact (@fold_1 m.(this)). Qed.
+  Lemma fold_1 : forall m (A : Type) (i : A) (f : key -> elt -> A -> A),
+      fold f m i = fold_left (fun a p => f (fst p) (snd p) a) (elements m) i.
+  Proof. intros m; apply Raw.fold_1. Qed.
 
-  Lemma _equal_1 : forall m m', _Equivb m m' -> _equal m m' = true.
-  Proof. intros m m'; exact (@equal_1 m.(this) m.(NoDup) m'.(this) m'.(NoDup)). Qed.
-  Lemma _equal_2 : forall m m', _equal m m' = true -> _Equivb m m'.
-  Proof. intros m m'; exact (@equal_2 m.(this) m.(NoDup) m'.(this) m'.(NoDup)). Qed.
+  Lemma equal_1 : forall m m', Equivb m m' -> equal m m' = true.
+  Proof. intros m m'; apply Raw.equal_1; auto. apply m.(sorted). apply  m'.(sorted). Qed.
+  Lemma equal_2 : forall m m', equal m m' = true -> Equivb m m'.
+  Proof. intros m m'; apply Raw.equal_2; auto. apply m.(sorted). apply  m'.(sorted). Qed.
+
+
+
+
+  Fixpoint eq_list (m m' : list (key * elt)) : Prop :=
+    match m, m' with
+    | nil, nil => True
+    | (x,e)::l, (x',e')::l' =>
+      match compare x x' with
+      | EQ _ => eq e e' /\ eq_list l l'
+      | _       => False
+      end
+    | _, _ => False
+    end.
+
+  Definition eq m m' := eq_list m.(this) m'.(this).
+
+  Lemma eq_equal : forall m m', eq m m' <-> equal m m' = true.
+  Proof.
+    intros (l,Hl); induction l.
+    intros (l',Hl'); unfold eq; simpl.
+    destruct l'; unfold equal; simpl; intuition.
+    intros (l',Hl'); unfold eq.
+    destruct l'.
+    destruct a; unfold equal; simpl; intuition.
+    destruct a as (x,e).
+    destruct p as (x',e').
+    unfold equal; simpl.
+    destruct (compare x x') as [Hlt|Heq|Hlt]; simpl; intuition.
+    unfold cmp at 1.
+    case (compare e e');
+    subst; intro HH; try (apply lt_not_eq in HH; now contradict HH);
+    clear HH; simpl.
+    inversion_clear Hl.
+    inversion_clear Hl'.
+    destruct (IHl H (Build_slist H2)).
+    unfold equal, eq in H5; simpl in H5; auto.
+    destruct (andb_prop _ _ H); clear H.
+    generalize H0; unfold cmp.
+    case (compare e e');
+    subst; intro HH; try (apply lt_not_eq in HH; now contradict HH);
+      auto; intro; discriminate.
+    destruct (andb_prop _ _ H); clear H.
+    inversion_clear Hl.
+    inversion_clear Hl'.
+    destruct (IHl H (Build_slist H3)).
+    unfold equal, eq in H6; simpl in H6; auto.
+  Qed.
+
+  Lemma eq_1 : forall m m', Equivb m m' -> eq m m'.
+  Proof.
+    intros.
+    generalize (@equal_1 m m').
+    generalize (@eq_equal m m').
+    intuition.
+  Qed.
+
+  Lemma eq_2 : forall m m', eq m m' -> Equivb m m'.
+  Proof.
+    intros.
+    generalize (@equal_2 m m').
+    generalize (@eq_equal m m').
+    intuition.
+  Qed.
+
+  Lemma eqfarray_refl : forall m : farray, eq m m.
+  Proof.
+    intros (m,Hm); induction m; unfold eq; simpl; auto.
+    destruct a.
+    destruct (compare k k) as [Hlt|Heq|Hlt]; auto.
+    apply lt_not_eq in Hlt. auto.
+    split.
+    apply eq_refl.
+    inversion_clear Hm.
+    apply (IHm H).
+    apply lt_not_eq in Hlt. auto.
+  Qed.
+
+  Lemma eqfarray_sym : forall m1 m2 : farray, eq m1 m2 -> eq m2 m1.
+  Proof.
+    intros (m,Hm); induction m;
+      intros (m', Hm'); destruct m'; unfold eq; simpl;
+        try destruct a as (x,e); try destruct p as (x',e'); auto.
+    destruct (compare x x')  as [Hlt|Heq|Hlt]; try easy.
+    inversion_clear Hm; inversion_clear Hm'.
+    intro. destruct H3.
+    subst.
+    case (compare x' x');
+    subst; intro HH; try (apply lt_not_eq in HH; now contradict HH).
+    split; auto.
+    apply (IHm H (Build_slist H1)); auto.
+  Qed.
+
+  Lemma eqfarray_trans : forall m1 m2 m3 : farray, eq m1 m2 -> eq m2 m3 -> eq m1 m3.
+  Proof.
+    intros (m1,Hm1); induction m1;
+      intros (m2, Hm2); destruct m2;
+        intros (m3, Hm3); destruct m3; unfold eq; simpl;
+          try destruct a as (x,e);
+          try destruct p as (x',e');
+          try destruct p0 as (x'',e''); try contradiction; auto.
+    destruct (compare x x') as [Hlt|Heq|Hlt];
+      destruct (compare x' x'') as [Hlt'|Heq'|Hlt']; try easy.
+    intros; destruct H, H0;  subst.
+    case (compare x'' x'');
+    subst; intro HH; try (apply lt_not_eq in HH; now contradict HH).
+    split; auto.
+    inversion_clear Hm1; inversion_clear Hm2; inversion_clear Hm3.
+    apply (IHm1 H (Build_slist H3) (Build_slist H5)); intuition.
+  Qed.
+
+
+
+  Fixpoint lt_list (m m' : list (key * elt)) : Prop :=
+    match m, m' with
+    | nil, nil => False
+    | nil, _  => True
+    | _, nil  => False
+    | (x,e)::l, (x',e')::l' =>
+      match compare x x' with
+      | LT _ => True
+      | GT _ => False
+      | EQ _ => lt e e' \/ (e = e' /\ lt_list l l')
+      end
+    end.
+
+  Definition lt_farray m m' := lt_list m.(this) m'.(this).
+
+  
+  Lemma lt_farray_trans : forall m1 m2 m3 : farray,
+      lt_farray m1 m2 -> lt_farray m2 m3 -> lt_farray m1 m3.
+  Proof.
+    intros (m1,Hm1); induction m1;
+      intros (m2, Hm2); destruct m2;
+        intros (m3, Hm3); destruct m3; unfold lt_farray; simpl;
+          try destruct a as (x,e);
+          try destruct p as (x',e');
+          try destruct p0 as (x'',e''); try contradiction; auto.
+    destruct (compare x x') as [Hlt|Heq|Hlt];
+      destruct (compare x' x'') as [Hlt'|Heq'|Hlt'];
+      destruct (compare x x'') as [Hlt''|Heq''|Hlt'']; intros; subst; auto; try easy.
+    apply (lt_trans x') in Hlt; apply lt_not_eq in Hlt.
+    now contradict Hlt. auto.
+    apply (lt_trans x') in Hlt; apply lt_not_eq in Hlt.
+    now contradict Hlt.
+    apply (lt_trans _ x'') ; auto.
+    apply lt_not_eq in Hlt. now contradict Hlt.
+    apply (lt_trans x'') in Hlt; apply lt_not_eq in Hlt.
+    now contradict Hlt. auto.
+    subst.
+    apply lt_not_eq in Hlt'. now contradict Hlt'.
+    apply (lt_trans x'') in Hlt'; apply lt_not_eq in Hlt'.
+    now contradict Hlt'. auto.
+    destruct H, H0.
+    left; apply lt_trans with e'; auto.
+    left. destruct H0. subst; auto.
+    left. destruct H. subst; auto.
+    right. destruct H, H0. subst; split; auto.
+    inversion_clear Hm1; inversion_clear Hm2; inversion_clear Hm3.
+    apply (IHm1 H (Build_slist H3) (Build_slist H5)); intuition.
+    apply lt_not_eq in Hlt''. now contradict Hlt''.
+  Qed.
+
+  Lemma lt_farray_not_eq : forall m1 m2 : farray, lt_farray m1 m2 -> ~ eq m1 m2.
+  Proof.
+    intros (m1,Hm1); induction m1;
+      intros (m2, Hm2); destruct m2; unfold eq, lt; simpl;
+        try destruct a as (x,e);
+        try destruct p as (x',e'); try contradiction; auto.
+    destruct (compare x x') as [Hlt|Heq|Hlt]; auto.
+    intuition.
+    inversion_clear Hm1; inversion_clear Hm2.
+    subst.
+    apply (IHm1 H0 (Build_slist H4)); intuition.
+    unfold lt_farray in *.
+    simpl in H.
+    case (compare x' x') in *.
+    apply lt_not_eq in l. now contradict l.
+    destruct H.
+    apply lt_not_eq in H. now contradict H.
+    destruct H.
+    auto.
+    apply lt_not_eq in l. now contradict l.
+  Qed.
+
+  Definition compare_farray : forall m1 m2, Compare lt_farray eq m1 m2.
+  Proof.
+    intros (m1,Hm1); induction m1;
+      intros (m2, Hm2); destruct m2;
+        [ apply EQ | apply LT | apply GT | ]; auto.
+    (* cmp_solve. *)
+    unfold eq. simpl; auto.
+    unfold lt_farray. simpl; auto.
+    unfold lt_farray. simpl; auto.
+    destruct a as (x,e); destruct p as (x',e').
+    destruct (compare x x');
+      [ apply LT | | apply GT ].
+    unfold lt_farray. simpl.
+    destruct (compare x x'); auto.
+    subst. apply lt_not_eq in l; now contradict l.
+    apply (lt_trans x') in l; auto. subst. apply lt_not_eq in l; now contradict l.
+    (* subst. *)
+    destruct (compare e e');
+      [ apply LT | | apply GT ].
+    unfold lt_farray. simpl.
+    destruct (compare x x'); auto; try (subst; apply lt_not_eq in l0; now contradict l0).
+    assert (Hm11 : sort (Raw.ltk key_ord) m1).
+    inversion_clear Hm1; auto.
+    assert (Hm22 : sort (Raw.ltk key_ord) m2).
+    inversion_clear Hm2; auto.
+    destruct (IHm1 Hm11 (Build_slist Hm22));
+      [ apply LT | apply EQ | apply GT ].
+    unfold lt_farray in *. simpl.
+    destruct (compare x x'); auto; try (subst; apply lt_not_eq in l0; now contradict l0).
+    unfold eq in *. simpl.
+    destruct (compare x x'); auto; try (subst; apply lt_not_eq in l; now contradict l).
+    unfold lt_farray in *. simpl.
+    destruct (compare x' x); auto; try (subst; apply lt_not_eq in l0; now contradict l0).
+    unfold lt_farray in *. simpl.
+    destruct (compare x' x); auto; try (subst; apply lt_not_eq in l0; now contradict l0).
+    unfold lt_farray in *. simpl.
+    destruct (compare x' x); auto; try (subst; apply lt_not_eq in l; now contradict l).
+    apply (lt_trans x) in l; auto. subst. apply lt_not_eq in l; now contradict l.
+  Qed.
+  (* TODO *)
 
   
   
@@ -679,27 +1293,27 @@ Section Array.
     symmetry; rewrite <- H; auto.
   Qed.
 
-  Lemma find_mapsto_iff : forall m x e, _MapsTo x e m <-> _find x m = Some e.
+  Lemma find_mapsto_iff : forall m x e, MapsTo x e m <-> find x m = Some e.
   Proof.
-    split; [apply _find_1|apply _find_2].
+    split; [apply find_1|apply find_2].
   Qed.
 
   Lemma add_neq_mapsto_iff : forall m x y e e',
-      x <> y -> (_MapsTo y e' (_add x e m)  <-> _MapsTo y e' m).
+      x <> y -> (MapsTo y e' (add x e m)  <-> MapsTo y e' m).
   Proof.
-    split; [apply _add_3|apply _add_2]; auto.
+    split; [apply add_3|apply add_2]; auto.
   Qed.
 
 
- Lemma add_eq_o : forall m x y e,
-      x = y -> _find y (_add x e m) = Some e.
+  Lemma add_eq_o : forall m x y e,
+      x = y -> find y (add x e m) = Some e.
   Proof. intros.
-    apply _find_1.
-    apply _add_1. auto.
-Qed.
+    apply find_1.
+    apply add_1. auto.
+  Qed.
 
   Lemma add_neq_o : forall m x y e,
-      ~ x = y -> _find y (_add x e m) = _find y m.
+      ~ x = y -> find y (add x e m) = find y m.
   Proof.
     intros. rewrite eq_option_alt. intro e'. rewrite <- 2 find_mapsto_iff.
     apply add_neq_mapsto_iff; auto.
@@ -708,20 +1322,19 @@ Qed.
 
 
 
-
   Lemma MapsTo_fun : forall m x (e e':elt),
-      _MapsTo x e m -> _MapsTo x e' m -> e=e'.
+      MapsTo x e m -> MapsTo x e' m -> e=e'.
   Proof.
     intros.
-    generalize (_find_1 H) (_find_1 H0); clear H H0.
+    generalize (find_1 H) (find_1 H0); clear H H0.
     intros; rewrite H in H0; injection H0; auto.
   Qed.
 
 
   (** Another characterisation of [Equal] *)
 
-  Lemma Equal_mapsto_iff : forall m1 m2 : _farray,
-      _Equal m1 m2 <-> (forall k e, _MapsTo k e m1 <-> _MapsTo k e m2).
+  Lemma Equal_mapsto_iff : forall m1 m2 : farray,
+      Equal m1 m2 <-> (forall k e, MapsTo k e m1 <-> MapsTo k e m2).
   Proof.
     intros m1 m2. split; [intros Heq k e|intros Hiff].
     rewrite 2 find_mapsto_iff, Heq. split; auto.
@@ -733,50 +1346,49 @@ Qed.
 
   (** First, [Equal] is [Equiv] with Leibniz on elements. *)
 
-  Lemma Equal_Equiv : forall (m m' : _farray),
-      _Equal m m' <-> _Equiv m m'.
+  Lemma Equal_Equiv : forall (m m' : farray),
+      Equal m m' <-> Equiv m m'.
   Proof.
     intros. rewrite Equal_mapsto_iff. split; intros.
     split.
-    split; intros (e,Hin); exists e; unfold _MapsTo in H; [rewrite <- H|rewrite H]; auto.
+    split; intros (e,Hin); exists e; unfold MapsTo in H; [rewrite <- H|rewrite H]; auto.
     intros; apply MapsTo_fun with m k; auto; rewrite H; auto.
     split; intros H'.
     destruct H.
-    assert (Hin : _In k m') by (rewrite <- H; exists e; auto).
+    assert (Hin : In k m') by (rewrite <- H; exists e; auto).
     destruct Hin as (e',He').
     rewrite (H0 k e e'); auto.
     destruct H.
-    assert (Hin : _In k m) by (rewrite H; exists e; auto).
+    assert (Hin : In k m) by (rewrite H; exists e; auto).
     destruct Hin as (e',He').
     rewrite <- (H0 k e' e); auto.
   Qed.
 
-  Lemma Equiv_Equivb : forall m m', _Equiv m m' <-> _Equivb m m'.
+  Lemma Equiv_Equivb : forall m m', Equiv m m' <-> Equivb m m'.
   Proof.
-    unfold _Equivb, _Equiv, Equivb; intuition.
-    rewrite eqb_elt_eq; apply H1 with k; unfold _MapsTo; auto.
-    rewrite <- eqb_elt_eq; apply H1 with k; unfold _MapsTo; auto.
+    unfold Equiv, Equivb, Raw.Equivb, cmp; intuition; specialize (H1 k e e' H H2).
+    destruct (compare e e'); auto; apply lt_not_eq in l; auto.
+    destruct (compare e e'); auto; now contradict H1.
   Qed.
 
 
   (** Composition of the two last results: relation between [Equal]
     and [Equivb]. *)
 
-  Lemma Equal_Equivb : forall (m m':_farray), _Equal m m' <-> _Equivb m m'.
+  Lemma Equal_Equivb : forall (m m':farray), Equal m m' <-> Equivb m m'.
   Proof.
     intros; rewrite Equal_Equiv.
     apply Equiv_Equivb; auto.
   Qed.
-
   
 
   (** * Functional arrays *)
 
   
-  Definition select (a: _farray) (i: key) : option elt := _find i a.
+  Definition select (a: farray) (i: key) : option elt := find i a.
 
 
-  Definition store (a: _farray) (i: key) (v: elt) : _farray := _add i v a.
+  Definition store (a: farray) (i: key) (v: elt) : farray := add i v a.
 
 
   Lemma read_over_same_write : forall a i j v, i = j -> select (store a i v) j = Some v.
@@ -798,16 +1410,16 @@ Qed.
 
   (* TODO *)
   Lemma find_ext_dec:
-    (forall m1 m2: _farray, _Equal m1 m2 -> (_equal m1 m2) = true).
+    (forall m1 m2: farray, Equal m1 m2 -> (equal m1 m2) = true).
   Proof. intros.
     apply Equal_Equivb in H.
-    apply _equal_1.
+    apply equal_1.
     exact H.
   Qed.
 
 
   Lemma extensionnality : forall a b,
-      (forall i, select a i = select b i) -> _equal a b = true.
+      (forall i, select a i = select b i) -> equal a b = true.
   Proof.
     intros.
     unfold select in H.
@@ -815,13 +1427,30 @@ Qed.
     exact H.
   Qed.
 
-  Definition eq a b := _equal a b = true.
+  Require Import ProofIrrelevance.
   
-  Lemma equal_eq : forall a b, _equal a b = true -> eq a b.
-  Proof. unfold eq. auto. Qed.
+  Lemma equal_eq : forall a b, equal a b = true -> a = b.
+  Proof. intros. apply eq_equal in H.
+    destruct a as (a, asort), b as (b, bsort).
+    unfold eq in H.
+    revert b bsort H.
+    induction a; intros; destruct b.
+    apply f_equal. apply proof_irrelevance.
+    simpl in H. now contradict H.
+    simpl in H. destruct a; now contradict H.
+    simpl in H. destruct a, p.
+    destruct (compare k k0); auto; try (now contradict H).
+    destruct H.
+    subst.
+    inversion_clear asort.
+    inversion_clear bsort.
+    specialize (IHa H b H2 H0).
+    inversion IHa. subst.
+    apply f_equal.  apply proof_irrelevance.
+ Qed.
 
   
-End Array.
+End FArray.
 
 
 (* 
